WebAssembly/Wasm_Base_Defs.thy
@@ -6,6 +6,7 @@ theory Wasm_Base_Defs
     Wasm_Type_Abs
     Wasm_Type_Word
     Word_Lib.Rsplit
+    "../libs/More_More_Word"
 begin
 
 text\<open>
@@ -164,66 +165,12 @@ lift_definition wasm_extend_s :: "i32 \<Rightarrow> i64" is "Word.scast" .
 
 (* int byte encoding *)
 
-fun bin_rsplit_rev :: "nat \<Rightarrow> nat \<Rightarrow> int \<Rightarrow> int list"
-  where "bin_rsplit_rev n m c =
-    (if m = 0 \<or> n = 0 then []
-     else
-      let (a, b) = bin_split n c
-      in b # bin_rsplit_rev n (m - n) a)"
+lift_definition serialise_i32 :: "i32 \<Rightarrow> bytes" is "(map Abs_uint8')\<circ>word_rsplit_rev" .
+lift_definition serialise_i64 :: "i64 \<Rightarrow> bytes" is "(map Abs_uint8')\<circ>word_rsplit_rev" .
 
-lemma bin_rsplit_rev_is:
-  "(rev acc)@(bin_rsplit_rev n m c) = rev (bin_rsplit_aux n m c acc)"
-proof (induction n m c arbitrary: acc rule: bin_rsplit_rev.induct)
-  case (1 n m c)
-  consider (1) "m = 0 \<or> n = 0" | (2) "\<not>(m = 0 \<or> n = 0)"
-    by blast
-  thus ?case
-  proof (cases)
-    case 1
-    thus ?thesis
-      by fastforce
-  next
-    case 2
-    obtain a b where a:"(a,b) = bin_split n c"
-      by simp
-    have "rev (b # acc) @ bin_rsplit_rev n (m - n) a =
-            rev (bin_rsplit_aux n (m - n) a (b # acc))"
-      using 2 1 a
-      by blast
-    thus ?thesis
-      using 2 a bin_rsplit_aux.elims
-      by fastforce
-  qed
-qed
-
-definition word_rsplit_rev :: "'a::len word \<Rightarrow> 'b::len word list"
-  where "word_rsplit_rev w = map word_of_int (bin_rsplit_rev (LENGTH('b)) (LENGTH('a)) (uint w))"
-
-lemma word_rsplit_rev_is: "word_rsplit_rev = rev \<circ> word_rsplit"
-  using bin_rsplit_rev_is
-  unfolding word_rsplit_def bin_rsplit_def word_rsplit_rev_def comp_def
-  by (metis (no_types, hide_lams) append_Nil fst_conv rev.simps(1) rev_map snd_conv)
-
-lift_definition serialise_i32 :: "i32 \<Rightarrow> bytes" is "word_rsplit_rev" .
-lift_definition serialise_i64 :: "i64 \<Rightarrow> bytes" is "word_rsplit_rev" .
-
-definition word_rcat_rev :: \<open>'a::len word list \<Rightarrow> 'b::len word\<close>
-  where \<open>word_rcat_rev = word_of_int \<circ> horner_sum uint (2 ^ LENGTH('a))\<close>
-
-lemma word_rcat_rev_is: "word_rcat_rev = word_rcat \<circ> rev"
-  unfolding word_rcat_def word_rcat_rev_def comp_def
-  by simp
-
-lemma word_rcat_rsplit_rev: "word_rcat_rev (word_rsplit_rev w) = w"
-  using word_rcat_rsplit[of w]
-  by (simp add: word_rcat_rev_is word_rsplit_rev_is)
-
-(* For some reason declaring these in two stages makes code extraction work better *)
-lift_definition deserialise_i32_aux :: "8 word list \<Rightarrow> i32" is "(\<lambda>x :: (8 word list). (word_rcat_rev x))" .
-lift_definition deserialise_i64_aux :: "8 word list \<Rightarrow> i64" is "(\<lambda>x :: (8 word list). (word_rcat_rev x))" .
-
-lift_definition deserialise_i32 :: "bytes \<Rightarrow> i32" is deserialise_i32_aux .
-lift_definition deserialise_i64 :: "bytes \<Rightarrow> i64" is "deserialise_i64_aux" .
+(* TODO: check code extraction works here *)
+lift_definition deserialise_i32 :: "bytes \<Rightarrow> i32" is "word_rcat_rev\<circ>(map Rep_uint8')" .
+lift_definition deserialise_i64 :: "bytes \<Rightarrow> i64" is "word_rcat_rev\<circ>(map Rep_uint8')" .
 
 lift_definition wasm_bool :: "bool \<Rightarrow> i32" is "(\<lambda>b. if b then 1 else 0)" .
 lift_definition  int32_minus_one :: i32 is "max_word" .
@@ -247,7 +194,9 @@ definition load :: "mem \<Rightarrow> nat \<Rightarrow> off \<Rightarrow> nat \<
 
 definition sign_extend :: "sx \<Rightarrow> nat \<Rightarrow> bytes \<Rightarrow> bytes" where
   "sign_extend sx l bytes = (let msb = msb_byte (msbyte bytes) in
-                          let byte = (case sx of U \<Rightarrow> zero_byte | S \<Rightarrow> if msb then negone_byte else zero_byte) in
+                          let byte = (case sx of
+                                        U \<Rightarrow> zero_byte
+                                      | S \<Rightarrow> if msb then negone_byte else zero_byte) in
                           bytes_takefill byte l bytes)"
 
 definition load_packed :: "sx \<Rightarrow> mem \<Rightarrow> nat \<Rightarrow> off \<Rightarrow> nat \<Rightarrow> nat \<Rightarrow> bytes option" where
