WebAssembly/Wasm_Interpreter_Monad_Properties.thy
@@ -1,9 +1,164 @@
-theory Wasm_Interpreter_Monad_Properties imports "../libs/List_Assn" Wasm_Interpreter_Monad begin
+theory Wasm_Interpreter_Monad_Properties imports "../libs/Misc_Generic_Lemmas" "../libs/List_Assn" Wasm_Interpreter_Monad begin
 
-term app_s_f_v_s_mem_size_m
+
+lemma load_f32_from_ui32_bs:
+  assumes "length bs \<le> 4"
+  shows "(serialise_i32 (i32_impl_abs (Abs_uint32' (word_rcat_rev (map Rep_uint8' bs))))) = takefill 0 4 bs"
+proof -
+  have 1:"(word_rsplit_rev::32 word \<Rightarrow> _) (word_rcat_rev (takefill 0 4 (map Rep_uint8 bs))) = takefill 0 4 (map Rep_uint8 bs)"
+    using word_split_rcat_rev_size assms
+    by (force simp add: word_size)
+  have 2:"Abs_uint8' \<circ> Rep_uint8 = id"
+    unfolding Abs_uint8'_def map_fun_def
+    by (simp add: Rep_uint8_inverse fun_comp_eq_conv)
+  have 3:"(word_rcat_rev :: _ \<Rightarrow> 32 word) (map Rep_uint8 bs) = (word_rcat_rev :: _ \<Rightarrow> 32 word) (takefill 0 4 (map Rep_uint8 bs))"
+    using word_rcat_rev_is_word_rcat_rev_takefill[of 4 "(map Rep_uint8 bs)"]
+    apply standard
+    apply (auto simp add: assms)
+    done
+  have 4: "(takefill 0 4 (map Rep_uint8 bs)) = (map Rep_uint8 (takefill 0 4 bs))"
+    unfolding map_takefill
+    by (simp add: zero_uint8.rep_eq)
+  show ?thesis
+    using 1 2 3 4
+    unfolding serialise_i32_def i32_impl_abs_def
+    by (auto simp add: I32.rep_abs Abs_uint32'.abs_eq Abs_uint32_inverse)
+qed
+
+lemma load_f64_from_ui64_bs:
+  assumes "length bs \<le> 8"
+  shows "(serialise_i64 (i64_impl_abs (Abs_uint64' (word_rcat_rev (map Rep_uint8' bs))))) = takefill 0 8 bs"
+proof -
+  have 1:"(word_rsplit_rev::64 word \<Rightarrow> _) (word_rcat_rev (takefill 0 8 (map Rep_uint8 bs))) = takefill 0 8 (map Rep_uint8 bs)"
+    using word_split_rcat_rev_size assms
+    by (force simp add: word_size)
+  have 2:"Abs_uint8' \<circ> Rep_uint8 = id"
+    unfolding Abs_uint8'_def map_fun_def
+    by (simp add: Rep_uint8_inverse fun_comp_eq_conv)
+  have 3:"(word_rcat_rev :: _ \<Rightarrow> 64 word) (map Rep_uint8 bs) = (word_rcat_rev :: _ \<Rightarrow> 64 word) (takefill 0 8 (map Rep_uint8 bs))"
+    using word_rcat_rev_is_word_rcat_rev_takefill[of 8 "(map Rep_uint8 bs)"]
+    apply standard
+    apply (auto simp add: assms)
+    done
+  have 4: "(takefill 0 8 (map Rep_uint8 bs)) = (map Rep_uint8 (takefill 0 8 bs))"
+    unfolding map_takefill
+    by (simp add: zero_uint8.rep_eq)
+  show ?thesis
+    using 1 2 3 4
+    unfolding serialise_i64_def i64_impl_abs_def
+    by (auto simp add: I64.rep_abs Abs_uint64'.abs_eq Abs_uint64_inverse)
+qed
+
+lemma word_list_sign_extend_Rep_uint8:
+  assumes "length bs > 0"
+  shows "(word_list_sign_extend n (map Rep_uint8' bs)) = map Rep_uint8' (sign_extend S n bs)"
+proof -
+  have "msb (last bs) = (msb (last (map Rep_uint8 bs)))"
+    using assms
+    apply (induction bs)
+    apply (simp_all add: msb_uint8.rep_eq)
+    done
+  thus ?thesis
+  unfolding msb_byte_def msbyte_def word_list_sign_extend_def sign_extend_def negone_byte_def zero_byte_def bytes_takefill_def
+  by (simp add: map_takefill one_uint8.rep_eq uminus_uint8.rep_eq zero_uint8.rep_eq)
+qed
+
+lemma load_f32_from_si32_bs:
+  assumes "length bs > 0" "length bs \<le> 4"
+  shows "(serialise_i32 (i32_impl_abs (Abs_uint32' (word_rcat_rev (word_list_sign_extend 4 (map Rep_uint8' bs)))))) = sign_extend S 4 bs"
+proof -
+  have 1:"
+     ((word_rsplit_rev :: 32 word \<Rightarrow> _)
+       ((word_rcat_rev)
+         (map Rep_uint8
+           (Wasm_Base_Defs.sign_extend S 4
+             bs)))) =
+    map Rep_uint8 (Wasm_Base_Defs.sign_extend S 4 bs)"
+    using word_split_rcat_rev_size[of "(map Rep_uint8 (Wasm_Base_Defs.sign_extend S 4 bs))"] assms
+    by (force simp add: word_size sign_extend_def bytes_takefill_def)
+  have 2:"Abs_uint8' \<circ> Rep_uint8 = id"
+    unfolding Abs_uint8'_def map_fun_def
+    by (simp add: Rep_uint8_inverse fun_comp_eq_conv)
+  have 3: "(takefill 0 4 (map Rep_uint8 bs)) = (map Rep_uint8 (takefill 0 4 bs))"
+    unfolding map_takefill
+    by (simp add: zero_uint8.rep_eq)
+  have "(serialise_i32 (i32_impl_abs (Abs_uint32' (word_rcat_rev (map Rep_uint8' (sign_extend S 4 bs)))))) = sign_extend S 4 bs"
+    using 2 3
+    unfolding serialise_i32_def i32_impl_abs_def
+    by (auto simp add: 1 I32.rep_abs Abs_uint32'.abs_eq Abs_uint32_inverse)
+  thus ?thesis
+    using word_list_sign_extend_Rep_uint8 assms(1)
+    by auto
+qed
+
+lemma load_f64_from_si64_bs:
+  assumes "length bs > 0" "length bs \<le> 8"
+  shows "(serialise_i64 (i64_impl_abs (Abs_uint64' (word_rcat_rev (word_list_sign_extend 8 (map Rep_uint8' bs)))))) = sign_extend S 8 bs"
+proof -
+  have 1:"
+     ((word_rsplit_rev :: 64 word \<Rightarrow> _)
+       ((word_rcat_rev)
+         (map Rep_uint8
+           (Wasm_Base_Defs.sign_extend S 8
+             bs)))) =
+    map Rep_uint8 (Wasm_Base_Defs.sign_extend S 8 bs)"
+    using word_split_rcat_rev_size[of "(map Rep_uint8 (Wasm_Base_Defs.sign_extend S 8 bs))"] assms
+    by (force simp add: word_size sign_extend_def bytes_takefill_def)
+  have 2:"Abs_uint8' \<circ> Rep_uint8 = id"
+    unfolding Abs_uint8'_def map_fun_def
+    by (simp add: Rep_uint8_inverse fun_comp_eq_conv)
+  have 3: "(takefill 0 4 (map Rep_uint8 bs)) = (map Rep_uint8 (takefill 0 4 bs))"
+    unfolding map_takefill
+    by (simp add: zero_uint8.rep_eq)
+  have "(serialise_i64 (i64_impl_abs (Abs_uint64' (word_rcat_rev (map Rep_uint8' (sign_extend S 8 bs)))))) = sign_extend S 8 bs"
+    using 2 3
+    unfolding serialise_i64_def i64_impl_abs_def
+    by (auto simp add: 1 I64.rep_abs Abs_uint64'.abs_eq Abs_uint64_inverse)
+  thus ?thesis
+    using word_list_sign_extend_Rep_uint8 assms(1)
+    by auto
+qed
+
+lemma store_f32_to_i32_bs:
+  assumes "length bs = 4"
+  shows "(map Abs_uint8' (takefill (0::8 word) n (word_rsplit_rev (Rep_uint32' (i32_impl_rep (deserialise_i32 bs)))))) = takefill (0::uint8) n bs"
+proof -
+  have 1:"(((word_rsplit_rev :: 32 word \<Rightarrow> _)
+         (Rep_i32 (deserialise_i32 bs)))) = map Rep_uint8 bs"
+    using word_split_rcat_rev_size[of "(map Rep_uint8 bs)"] assms
+    unfolding deserialise_i32_def
+    by (force simp add: word_size Abs_i32_inverse)
+  have 2:"Abs_uint8' \<circ> Rep_uint8 = id"
+    unfolding Abs_uint8'_def map_fun_def
+    by (simp add: Rep_uint8_inverse fun_comp_eq_conv)
+  show ?thesis
+    using 1 2
+    unfolding i32_impl_rep_def
+    by (simp add: Abs_uint32_inverse map_takefill Abs_uint8'.abs_eq zero_uint8.abs_eq)
+qed
+
+lemma store_f64_to_i64_bs:
+  assumes "length bs = 8"
+  shows "(map Abs_uint8' (takefill (0::8 word) n (word_rsplit_rev (Rep_uint64' (i64_impl_rep (deserialise_i64 bs)))))) = takefill (0::uint8) n bs"
+proof -
+  have 1:"(((word_rsplit_rev :: 64 word \<Rightarrow> _)
+         (Rep_i64 (deserialise_i64 bs)))) = map Rep_uint8 bs"
+    using word_split_rcat_rev_size[of "(map Rep_uint8 bs)"] assms
+    unfolding deserialise_i64_def
+    by (force simp add: word_size Abs_i64_inverse)
+  have 2:"Abs_uint8' \<circ> Rep_uint8 = id"
+    unfolding Abs_uint8'_def map_fun_def
+    by (simp add: Rep_uint8_inverse fun_comp_eq_conv)
+  show ?thesis
+    using 1 2
+    unfolding i64_impl_rep_def
+    by (simp add: Abs_uint64_inverse map_takefill Abs_uint8'.abs_eq zero_uint8.abs_eq)
+qed
+  
+  term app_s_f_v_s_mem_size_m
 term app_s_f_v_s_mem_size
 
-definition "mem_m_assn \<equiv> \<lambda>(mr,mm) (mri,mmi). mri \<mapsto>\<^sub>a Rep_mem_rep mr * \<up>(mmi=mm)"
+definition "mem_m_assn \<equiv> \<lambda>(mr,mm) (mri,mmi). mri \<mapsto>\<^sub>b\<^sub>a Rep_mem_rep mr * \<up>(mmi=mm)"
 
 definition "inst_m_assn i ii \<equiv> 
     inst_m.types ii \<mapsto>\<^sub>a inst.types i
@@ -12,7 +167,7 @@ definition "inst_m_assn i ii \<equiv>
   * inst_m.mems  ii \<mapsto>\<^sub>a inst.mems  i 
   * inst_m.globs ii \<mapsto>\<^sub>a inst.globs i"
      
-lemma [sep_heap_rules]: "<mem_m_assn m mi> Array.len (fst mi) <\<lambda>r. mem_m_assn m mi * \<up>(r=length (Rep_mem_rep (fst m)))>"
+lemma [sep_heap_rules]: "<mem_m_assn m mi> len_byte_array (fst mi) <\<lambda>r. mem_m_assn m mi * \<up>(r=length (Rep_mem_rep (fst m)))>"
   unfolding mem_m_assn_def
   by (sep_auto split: prod.splits)
 
