libs/Byte_Array.thy
@@ -1,0 +1,267 @@
+theory Byte_Array
+  imports
+    Main
+    "Native_Word.Uint8"
+    "Native_Word.Uint32"
+    "Native_Word.Uint64"
+    "HOL-Imperative_HOL.Array"
+    "Array_Blit"
+    "More_More_Word"
+begin
+
+chapter \<open>Monadic byte arrays, geared towards OCaml's "bytes" type\<close>
+
+typedef byte_array = "UNIV :: (uint8 array) set" ..
+setup_lifting type_definition_byte_array
+declare Quotient_byte_array[transfer_rule]
+
+instance uint8 :: heap
+  apply standard
+  apply transfer
+  apply auto
+  done
+
+instance byte_array :: heap
+  apply standard
+  apply transfer
+  apply auto
+  done
+
+lift_definition
+  bl_assn :: "byte_array \<Rightarrow> uint8 list \<Rightarrow> assn" (infix "\<mapsto>\<^sub>b\<^sub>a" 82)
+  is "\<lambda>(r::uint8 array) (a::uint8 list). r\<mapsto>\<^sub>aa" .
+
+(* basic operations *)
+
+lift_definition new_zeroed_byte_array :: "nat \<Rightarrow> byte_array Heap" is
+  "\<lambda>n. Array.new n (0::uint8)" .
+
+lift_definition len_byte_array :: "byte_array \<Rightarrow> nat Heap" is
+  "Array.len :: uint8 array \<Rightarrow> nat Heap" .
+
+lift_definition blit_byte_array :: "byte_array \<Rightarrow> nat \<Rightarrow> byte_array \<Rightarrow> nat \<Rightarrow> nat \<Rightarrow> unit Heap" is
+  "blit :: uint8 array \<Rightarrow> nat \<Rightarrow> uint8 array \<Rightarrow> nat \<Rightarrow> nat \<Rightarrow> unit Heap" .
+
+definition grow_zeroed_byte_array :: "byte_array \<Rightarrow> nat \<Rightarrow> byte_array Heap" where
+  "grow_zeroed_byte_array a n \<equiv> do {
+    if n=0 then 
+      return a
+    else do {
+      l\<leftarrow>len_byte_array a;
+      a'\<leftarrow>new_zeroed_byte_array (l+n);
+      blit_byte_array a 0 a' 0 l;
+      return a'
+    }
+  }"
+
+lemma map_Heap_assn:
+  assumes
+    "inj f"
+    "
+    < P > 
+      c
+    <\<lambda>x. Q x>"
+  shows "
+    < P > 
+      map_Heap f c
+    <\<lambda>x. Q ((inv f) x)>"
+  using assms
+  unfolding hoare_triple_def
+  apply (cases c)
+  apply (simp add: Let_def run.simps)
+  apply (metis (no_types, lifting) inv_f_f)
+  done
+
+lemma map_Heap_byte_array:
+  assumes "
+    < P > 
+      c
+    <\<lambda>(x::uint8 array). Q x>"
+  shows "
+    < P > 
+      map_Heap Abs_byte_array c
+    <\<lambda>x. Q (Rep_byte_array x)>"
+proof -
+  have "inj Abs_byte_array"
+    by (metis Abs_byte_array_inverse UNIV_I inj_def)
+  moreover hence "inv Abs_byte_array = Rep_byte_array"
+    by (simp add: Rep_byte_array_inverse inj_imp_inv_eq)
+  ultimately show ?thesis
+    using map_Heap_assn assms
+    by metis
+qed
+
+lemma new_zeroed_byte_array_rule[sep_heap_rules]:
+  shows "
+    < emp > 
+      new_zeroed_byte_array n
+    <\<lambda>a'. a'\<mapsto>\<^sub>b\<^sub>a (replicate n 0)>"
+  using map_Heap_byte_array[OF new_rule]
+  unfolding new_zeroed_byte_array_def bl_assn_def
+  by sep_auto
+
+lemma len_byte_array_rule[sep_heap_rules]:
+  "<a \<mapsto>\<^sub>b\<^sub>a la>
+     len_byte_array a
+   <\<lambda>r. a \<mapsto>\<^sub>b\<^sub>a la * \<up>(r = length la)>"
+  using map_Heap_byte_array
+  unfolding len_byte_array_def bl_assn_def
+  by sep_auto
+
+lemma blit_byte_array_rule[sep_heap_rules]:
+  assumes LEN: "si+len \<le> length lsrc" "di+len \<le> length ldst"
+  shows
+  "< src \<mapsto>\<^sub>b\<^sub>a lsrc 
+    * dst \<mapsto>\<^sub>b\<^sub>a ldst >
+  blit_byte_array src si dst di len
+  <\<lambda>_. src \<mapsto>\<^sub>b\<^sub>a lsrc 
+    * dst \<mapsto>\<^sub>b\<^sub>a (take di ldst @ take len (drop si lsrc) @ drop (di+len) ldst)
+  >"
+  using map_Heap_byte_array assms
+  unfolding blit_byte_array_def bl_assn_def
+  by sep_auto
+
+lemma grow_zeroed_byte_array_rule[sep_heap_rules]:
+  shows "
+    < a\<mapsto>\<^sub>b\<^sub>ala > 
+      grow_zeroed_byte_array a n 
+    <\<lambda>a'. a'\<mapsto>\<^sub>b\<^sub>a (la @ replicate n 0)>\<^sub>t"
+  using map_Heap_byte_array
+  unfolding grow_zeroed_byte_array_def
+  by (sep_auto heap:len_byte_array_rule new_zeroed_byte_array_rule blit_byte_array_rule)
+
+(* loading and storing bytes *)
+
+lift_definition load_uint8 :: "byte_array \<Rightarrow> nat \<Rightarrow> uint8 Heap" is
+   "\<lambda>(a::uint8 array) n. Array.nth a n" .
+
+fun load_uint8_list :: "byte_array \<Rightarrow> nat \<Rightarrow> nat \<Rightarrow> uint8 list Heap" where
+  "load_uint8_list a n 0 = return []"
+| "load_uint8_list a n (Suc l) = do {
+     b\<leftarrow>load_uint8 a n;
+     bs\<leftarrow>load_uint8_list a (Suc n) l;
+     return (b#bs)
+   }"
+
+lift_definition store_uint8 :: "byte_array \<Rightarrow> nat \<Rightarrow> uint8 \<Rightarrow> unit Heap" is
+   "\<lambda>(a::uint8 array) n b. (do { Array.upd n b a; return () })" .
+
+fun store_uint8_list :: "byte_array \<Rightarrow> nat \<Rightarrow> uint8 list \<Rightarrow> unit Heap" where
+  "store_uint8_list a n [] = return ()"
+| "store_uint8_list a n (b#bs) = do {
+     store_uint8 a n b;
+     store_uint8_list a (Suc n) bs
+   }"
+
+(* loading and storing uint32 *)
+
+definition load_uint32_of_uint8 :: "byte_array \<Rightarrow> nat \<Rightarrow> uint32 Heap" where
+  "load_uint32_of_uint8 a n \<equiv> do {
+     b\<leftarrow>load_uint8 a n;
+     return (Abs_uint32' (ucast (Rep_uint8' b)))
+  }"
+
+definition load_uint32_of_sint8 :: "byte_array \<Rightarrow> nat \<Rightarrow> uint32 Heap" where
+  "load_uint32_of_sint8 a n \<equiv> do {
+     b\<leftarrow>load_uint8 a n;
+     return (Abs_uint32' (scast (Rep_uint8' b)))
+  }"
+
+definition load_uint32_of_uint16 :: "byte_array \<Rightarrow> nat \<Rightarrow> uint32 Heap" where
+  "load_uint32_of_uint16 a n \<equiv> do {
+     bs\<leftarrow>load_uint8_list a n 2;
+     return (Abs_uint32' (word_rcat_rev (map Rep_uint8' bs)))
+  }"
+
+definition load_uint32_of_sint16 :: "byte_array \<Rightarrow> nat \<Rightarrow> uint32 Heap" where
+  "load_uint32_of_sint16 a n \<equiv> do {
+     bs\<leftarrow>load_uint8_list a n 2;
+     return (Abs_uint32' (word_rcat_rev (word_list_sign_extend 4 (map Rep_uint8' bs))))
+  }"
+
+definition load_uint32 :: "byte_array \<Rightarrow> nat \<Rightarrow> uint32 Heap" where
+  "load_uint32 a n \<equiv> do {
+     bs\<leftarrow>load_uint8_list a n 4;
+     return (Abs_uint32' (word_rcat_rev (map Rep_uint8' bs)))
+  }"
+
+definition store_uint8_of_uint32 :: "byte_array \<Rightarrow> nat \<Rightarrow> uint32 \<Rightarrow> unit Heap" where
+  "store_uint8_of_uint32 a n v \<equiv> do {
+     store_uint8_list a n (map Abs_uint8' (takefill (0::8 word) 1 (word_rsplit_rev (Rep_uint32' v))))
+  }"
+
+definition store_uint16_of_uint32 :: "byte_array \<Rightarrow> nat \<Rightarrow> uint32 \<Rightarrow> unit Heap" where
+  "store_uint16_of_uint32 a n v \<equiv> do {
+     store_uint8_list a n (map Abs_uint8' (takefill (0::8 word) 2 (word_rsplit_rev (Rep_uint32' v))))
+  }"
+
+definition store_uint32 :: "byte_array \<Rightarrow> nat \<Rightarrow> uint32 \<Rightarrow> unit Heap" where
+  "store_uint32 a n v \<equiv> do {
+     store_uint8_list a n (map Abs_uint8' (takefill (0::8 word) 4 (word_rsplit_rev (Rep_uint32' v))))
+  }"
+
+(* loading and storing uint64 *)
+
+definition load_uint64_of_uint8 :: "byte_array \<Rightarrow> nat \<Rightarrow> uint64 Heap" where
+  "load_uint64_of_uint8 a n \<equiv> do {
+     b\<leftarrow>load_uint8 a n;
+     return (Abs_uint64' (ucast (Rep_uint8' b)))
+  }"
+
+definition load_uint64_of_sint8 :: "byte_array \<Rightarrow> nat \<Rightarrow> uint64 Heap" where
+  "load_uint64_of_sint8 a n \<equiv> do {
+     b\<leftarrow>load_uint8 a n;
+     return (Abs_uint64' (scast (Rep_uint8' b)))
+  }"
+
+definition load_uint64_of_uint16 :: "byte_array \<Rightarrow> nat \<Rightarrow> uint64 Heap" where
+  "load_uint64_of_uint16 a n \<equiv> do {
+     bs\<leftarrow>load_uint8_list a n 2;
+     return (Abs_uint64' (word_rcat_rev (map Rep_uint8' bs)))
+  }"
+
+definition load_uint64_of_sint16 :: "byte_array \<Rightarrow> nat \<Rightarrow> uint64 Heap" where
+  "load_uint64_of_sint16 a n \<equiv> do {
+     bs\<leftarrow>load_uint8_list a n 2;
+     return (Abs_uint64' (word_rcat_rev (word_list_sign_extend 8 (map Rep_uint8' bs))))
+  }"
+
+definition load_uint64_of_uint32 :: "byte_array \<Rightarrow> nat \<Rightarrow> uint64 Heap" where
+  "load_uint64_of_uint32 a n \<equiv> do {
+     bs\<leftarrow>load_uint8_list a n 4;
+     return (Abs_uint64' (word_rcat_rev (map Rep_uint8' bs)))
+  }"
+
+definition load_uint64_of_sint32 :: "byte_array \<Rightarrow> nat \<Rightarrow> uint64 Heap" where
+  "load_uint64_of_sint32 a n \<equiv> do {
+     bs\<leftarrow>load_uint8_list a n 4;
+     return (Abs_uint64' (word_rcat_rev (word_list_sign_extend 8 (map Rep_uint8' bs))))
+  }"
+
+definition load_uint64 :: "byte_array \<Rightarrow> nat \<Rightarrow> uint64 Heap" where
+  "load_uint64 a n \<equiv> do {
+     bs\<leftarrow>load_uint8_list a n 8;
+     return (Abs_uint64' (word_rcat_rev (map Rep_uint8' bs)))
+  }"
+
+definition store_uint8_of_uint64 :: "byte_array \<Rightarrow> nat \<Rightarrow> uint64 \<Rightarrow> unit Heap" where
+  "store_uint8_of_uint64 a n v \<equiv> do {
+     store_uint8_list a n (map Abs_uint8' (takefill (0::8 word) 1 (word_rsplit_rev (Rep_uint64' v))))
+  }"
+
+definition store_uint16_of_uint64 :: "byte_array \<Rightarrow> nat \<Rightarrow> uint64 \<Rightarrow> unit Heap" where
+  "store_uint16_of_uint64 a n v \<equiv> do {
+     store_uint8_list a n (map Abs_uint8' (takefill (0::8 word) 2 (word_rsplit_rev (Rep_uint64' v))))
+  }"
+
+definition store_uint32_of_uint64 :: "byte_array \<Rightarrow> nat \<Rightarrow> uint64 \<Rightarrow> unit Heap" where
+  "store_uint32_of_uint64 a n v \<equiv> do {
+     store_uint8_list a n (map Abs_uint8' (takefill (0::8 word) 4 (word_rsplit_rev (Rep_uint64' v))))
+  }"
+
+definition store_uint64 :: "byte_array \<Rightarrow> nat \<Rightarrow> uint64 \<Rightarrow> unit Heap" where
+  "store_uint64 a n v \<equiv> do {
+     store_uint8_list a n (map Abs_uint8' (takefill (0::8 word) 8 (word_rsplit_rev (Rep_uint64' v))))
+  }"
+
+end
