libs/Misc_Generic_Lemmas.thy
@@ -1,0 +1,10 @@
+theory Misc_Generic_Lemmas imports Main Word_Lib.Reversed_Bit_Lists begin
+
+(* These lemmas are fairly generic and could be contributed back to their libs? *)
+
+lemma map_takefill:"(map f (takefill k n bs)) = (takefill (f k) n (map f bs))"
+  apply (induction n arbitrary: bs)
+  apply (simp_all split: list.splits)
+  done
+
+end
